src/Extraction/OrSigmalib/Extraction.v
@@ -2,5 +2,5 @@ From Stdlib Require Import Extraction
 ExtrOcamlBasic ExtrOcamlNativeString
 ExtrOcamlZBigInt ExtrOcamlNatBigInt.
 From Examples Require Import OrSigmaIns.
-Set Extraction Output Directory ".". 
+Set Extraction Output Directory ".".
 Separate Extraction OrSigmaIns.
